Work on state_app_unitProof

compiler/backend/passes/proofs/state_app_unitProofScript.sml
@@ -6,831 +6,459 @@
 open HolKernel Parse boolLib bossLib BasicProvers dep_rewrite;
 open stringTheory optionTheory sumTheory pairTheory listTheory alistTheory
      finite_mapTheory pred_setTheory rich_listTheory arithmeticTheory
-open pure_exp_lemmasTheory pure_miscTheory pure_configTheory
-     stateLangTheory;
+open pure_exp_lemmasTheory pure_miscTheory pure_configTheory state_cexpTheory
+     stateLangTheory state_app_unit_1ProofTheory state_app_unit_2ProofTheory;
 local open pure_semanticsTheory in end
 
 val _ = new_theory "state_app_unitProof";
 
-val _ = set_grammar_ancestry ["stateLang"];
+val _ = set_grammar_ancestry
+  ["stateLang","state_cexp","state_app_unit_1Proof","state_app_unit_2Proof"];
 
-Overload "app" = “λe1 e2. App AppOp [e1;e2]”;
+Overload "app" = “λe1 e2. App AppOp [e1;(e2:cexp)]”;
+Overload "Unit" = “App (Cons "") [] :cexp”;
 
-Inductive compile_rel:
+Inductive cexp1_rel:
 
-[~App_Unit:]
-  (compile_rel (n+1:num) x y ⇒
-  compile_rel n (app x Unit) y) ∧
+[~App_Lam:]
+  (cexp1_rel x y ⇒
+   cexp1_rel (app (Lam NONE x) Unit) y) ∧
 
-[~Lam_Unit:]
-  (compile_rel n x y ⇒
-  compile_rel (n+1) (Lam NONE x) y) ∧
+[~App_Let:]
+  (cexp1_rel x x1 ∧ cexp1_rel y y1 ⇒
+   cexp1_rel (app (Let x_opt x y) Unit)
+             (Let x_opt x1 (app y1 Unit))) ∧
+
+[~App_If:]
+  (cexp1_rel x x1 ∧ cexp1_rel y y1 ∧ cexp1_rel z z1 ⇒
+   cexp1_rel (app (If x y z) Unit)
+             (If x1 (app y1 Unit) (app z1 Unit))) ∧
+
+[~App_Letrec:]
+  (cexp1_rel y y1 ∧
+   MAP FST tfns = MAP FST sfns ∧
+   MAP (FST o SND) tfns = MAP (FST o SND) sfns ∧
+   LIST_REL cexp1_rel (MAP (SND o SND) tfns) (MAP (SND o SND) sfns) ⇒
+   cexp1_rel (app (Letrec tfns y) Unit)
+             (Letrec sfns (app y1 Unit))) ∧
 
 [~Var:]
-  compile_rel 0 (stateLang$Var v) (stateLang$Var v) ∧
+  cexp1_rel (state_cexp$Var v) (state_cexp$Var v) ∧
 
-[~Lam_SOME:]
-  (compile_rel 0 x y ⇒
-  compile_rel 0 (Lam ov x) (Lam ov y)) ∧
+[~Lam:]
+  (cexp1_rel x y ⇒
+  cexp1_rel (Lam ov x) (Lam ov y)) ∧
 
 [~Raise:]
-  (compile_rel 0 x y ⇒
-  compile_rel 0 (Raise x) (Raise y)) ∧
+  (cexp1_rel x y ⇒
+  cexp1_rel (Raise x) (Raise y)) ∧
 
 [~Handle:]
-  (compile_rel 0 x1 y1 ∧ compile_rel 0 x2 y2 ⇒
-  compile_rel 0 (Handle x1 v x2) (Handle y1 v y2)) ∧
+  (cexp1_rel x1 y1 ∧ cexp1_rel x2 y2 ⇒
+  cexp1_rel (Handle x1 v x2) (Handle y1 v y2)) ∧
 
 [~HandleApp:]
-  (compile_rel 0 x1 y1 ∧ compile_rel 0 x2 y2 ⇒
-  compile_rel 0 (HandleApp x1 x2) (HandleApp y1 y2)) ∧
+  (cexp1_rel x1 y1 ∧ cexp1_rel x2 y2 ⇒
+  cexp1_rel (HandleApp x1 x2) (HandleApp y1 y2)) ∧
 
 [~App:]
-  (LIST_REL (compile_rel 0) xs ys ⇒
-  compile_rel 0 (App op xs) (App op ys)) ∧
+  (LIST_REL (cexp1_rel) xs ys ⇒
+  cexp1_rel (App op xs) (App op ys)) ∧
 
 [~Letrec:]
   (∀tfns sfns te se.
     MAP FST tfns = MAP FST sfns ∧
-    LIST_REL (compile_rel 0) (MAP SND tfns) (MAP SND sfns) ∧
-    EVERY (λ(n,x). ∃v y. x = Lam v y) tfns ∧
-    compile_rel n te se ⇒
-    compile_rel n (Letrec tfns te) (Letrec sfns se)) ∧
+    MAP (FST o SND) tfns = MAP (FST o SND) sfns ∧
+    LIST_REL cexp1_rel (MAP (SND o SND) tfns) (MAP (SND o SND) sfns) ∧
+    cexp1_rel te se ⇒
+    cexp1_rel (Letrec tfns te) (Letrec sfns se)) ∧
 
 [~Let:]
-  (compile_rel 0 te1 se1 ∧
-   compile_rel n te2 se2 ⇒
-  compile_rel n (Let x_opt te1 te2) (Let x_opt se1 se2)) ∧
+  (cexp1_rel te1 se1 ∧
+   cexp1_rel te2 se2 ⇒
+  cexp1_rel (Let x_opt te1 te2) (Let x_opt se1 se2)) ∧
 
 [~If:]
-  (compile_rel 0 te se ∧
-   compile_rel n te1 se1 ∧
-   compile_rel n te2 se2 ⇒
-  compile_rel n (If te te1 te2) (If se se1 se2)) ∧
+  (cexp1_rel te se ∧
+   cexp1_rel te1 se1 ∧
+   cexp1_rel te2 se2 ⇒
+  cexp1_rel (If te te1 te2) (If se se1 se2)) ∧
 
 [~Case:]
   (∀v te se tes ses.
-     compile_rel 0 te se ∧
+     cexp1_rel te se ∧
      MAP FST tes = MAP FST ses ∧
      MAP (FST o SND) tes = MAP (FST o SND) ses ∧
-     LIST_REL (compile_rel n) (MAP (SND o SND) tes) (MAP (SND o SND) ses) ⇒
-  compile_rel n (Case te v tes) (Case se v ses))
+     LIST_REL cexp1_rel (MAP (SND o SND) tes) (MAP (SND o SND) ses) ⇒
+  cexp1_rel (Case te v tes) (Case se v ses))
 
 End
 
-Inductive v_rel:
+Overload rel1 = “state_app_unit_1Proof$compile_rel”
+Overload rel2 = “state_app_unit_2Proof$compile_rel”
 
-[~Atom:]
-  (∀a.
-     v_rel (Atom a) (Atom a)) ∧
-
-[~Constructor:]
-  (∀s tvs svs.
-     LIST_REL v_rel tvs svs ⇒
-     v_rel (Constructor s tvs) (Constructor s svs)) ∧
-
-[~Closure:]
-  (∀tenv senv te se n.
-     env_rel tenv senv ∧ compile_rel 0 te se ⇒
-     v_rel (Closure n tenv te) (Closure n senv se)) ∧
-
-[~Recclosure:]
-  (∀tfns sfns tenv senv n.
-     env_rel tenv senv ∧
-     LIST_REL (compile_rel 0) (MAP SND tfns) (MAP SND sfns) ∧
-     MAP FST tfns = MAP FST sfns ∧
-     EVERY (λ(n,x). ∃v y. x = Lam v y) tfns  ⇒
-     v_rel (Recclosure tfns tenv n)
-           (Recclosure sfns senv n)) ∧
-
-[env_rel:]
-  (∀tenv senv.
-     (∀(n:string) tv.
-       ALOOKUP tenv n = SOME tv ⇒
-       ∃sv. ALOOKUP senv n = SOME sv ∧ v_rel tv sv) ⇒
-     env_rel tenv senv)
-
-End
-
-Theorem env_rel_def = “env_rel tenv senv”
-  |> SIMP_CONV (srw_ss()) [Once v_rel_cases];
-
-Inductive cont_rel:
-  (∀n. n = 0 ⇒ cont_rel n [] []) ∧
-  (∀n tk sk.
-    cont_rel n tk sk ⇒
-    cont_rel (n+1:num) (AppK env AppOp [Constructor "" []] []::tk) sk) ∧
-  (∀n tk sk.
-    cont_rel n tk sk ∧ env_rel tenv senv ∧
-    compile_rel n te1 se1 ∧ compile_rel n te2 se2 ⇒
-    cont_rel 0 (IfK tenv te1 te2 :: tk)
-               (IfK senv se1 se2 :: sk)) ∧
-  (∀tenv senv op tvs svs tes ses sk tk.
-    cont_rel 0 tk sk ∧ env_rel tenv senv ∧
-    LIST_REL v_rel tvs svs ∧ LIST_REL (compile_rel 0) tes ses ⇒
-    cont_rel 0 (AppK tenv op tvs tes :: tk)
-               (AppK senv op svs ses :: sk)) ∧
-  (∀tenv senv n te se sk tk.
-    cont_rel m tk sk ∧ env_rel tenv senv ∧
-    compile_rel m te se ⇒
-    cont_rel 0 (LetK tenv n te :: tk)
-               (LetK senv n se :: sk)) ∧
-  (∀tenv senv n te se sk tk.
-    cont_rel 0 tk sk ∧ env_rel tenv senv ∧
-    compile_rel 0 te se ⇒
-    cont_rel 0 (HandleK tenv n te :: tk)
-               (HandleK senv n se :: sk)) ∧
-  (∀tenv senv te se sk tk.
-    cont_rel 0 tk sk ∧ env_rel tenv senv ∧
-    compile_rel 0 te se ⇒
-    cont_rel 0 (HandleAppK tenv te :: tk)
-               (HandleAppK senv se :: sk)) ∧
-  (∀sk tk.
-    cont_rel 0 tk sk ⇒
-    cont_rel 0 (RaiseK :: tk)
-               (RaiseK :: sk)) ∧
-  (∀sk tk v tenv senv.
-    cont_rel n tk sk ∧ env_rel tenv senv ∧
-    MAP FST tes = MAP FST ses ∧
-    MAP (FST o SND) tes = MAP (FST o SND) ses ∧
-    LIST_REL (compile_rel n) (MAP (SND o SND) tes) (MAP (SND o SND) ses) ⇒
-    cont_rel 0 (CaseK tenv v tes :: tk)
-               (CaseK senv v ses :: sk))
-End
-
-Inductive step_res_rel:
-  (v_rel v1 v2 ∧ cont_rel 0 tk sk ⇒
-   step_res_rel (Val v1) tk (Val v2) sk) ∧
-  (v_rel v1 v2 ∧ cont_rel 0 tk sk ⇒
-   step_res_rel (Exn v1) tk (Exn v2) sk) ∧
-  (step_res_rel Error tk Error sk) ∧
-  (compile_rel n e1 e2 ∧ env_rel env1 env2 ∧ cont_rel n tk sk ⇒
-   step_res_rel (Exp env1 e1) tk (Exp env2 e2) sk) ∧
-  (cont_rel 0 tk sk ⇒
-   step_res_rel (Action a b) tk (Action a b) sk)
-End
-
-Definition rec_env_def:
-  rec_env f env =
-    MAP (λ(fn,_). (fn,Recclosure f env fn)) f ++ env
-End
-
-Inductive snext_res_rel:
-  (OPTREL (LIST_REL (LIST_REL v_rel)) ts ss ∧ cont_rel 0 tk sk ⇒
-   snext_res_rel (Act x tk ts) (Act x sk ss)) ∧
-  (snext_res_rel Ret Ret) ∧
-  (snext_res_rel Div Div) ∧
-  (snext_res_rel Err Err)
-End
-
-Inductive insert_appk:
-  insert_appk tk (AppK env AppOp [Constructor "" []] []::tk) ∧
-  (insert_appk tk tk1 ⇒
-   insert_appk (IfK tenv te1 te2 :: tk)
-               (IfK tenv te1 te2 :: tk1)) ∧
-  (insert_appk tk tk1 ⇒
-   insert_appk (LetK tenv n te :: tk)
-               (LetK tenv n te :: tk1)) ∧
-  (insert_appk tk tk1 ⇒
-   insert_appk (CaseK tenv v tes :: tk)
-               (CaseK tenv v tes :: tk1))
-End
-
-Theorem cont_rel_insert_appk:
-  ∀n tk sk.
-    cont_rel (n+1) tk sk ⇒
-    ∃tk0. cont_rel n tk0 sk ∧ insert_appk tk0 tk
+Triviality LIST_REL_rel2_rel1:
+  ∀xs zs.
+    LIST_REL (λx z. cexp1_rel x z ∧ ∃y. rel2 (exp_of x) y ∧ rel1 y (exp_of z)) xs zs ⇒
+    ∃ys. LIST_REL rel2 (MAP exp_of xs) ys ∧ LIST_REL rel1 ys (MAP exp_of zs)
 Proof
-  Induct_on ‘tk’ \\ fs []
-  \\ simp [Once cont_rel_cases] \\ rw []
-  \\ first_x_assum $ irule_at Any
-  \\ simp [Once insert_appk_cases]
+  Induct \\ Cases_on ‘zs’ \\ fs [PULL_EXISTS]
+  \\ rw [] \\ res_tac \\ fs [] \\ metis_tac []
 QED
 
-Theorem env_rel_cons:
-  env_rel xs ys ∧ v_rel x y ⇒
-  env_rel ((n,x)::xs) ((n,y)::ys)
+Theorem cexp1_rel_thm:
+  ∀x z. cexp1_rel x z ⇒ ∃y. rel2 (exp_of x) y ∧ rel1 y (exp_of z)
 Proof
-  rw [env_rel_def] \\ rw [] \\ fs []
+  Induct_on ‘cexp1_rel’ \\ rpt strip_tac \\ simp []
+  >-
+   (irule_at Any state_app_unit_1ProofTheory.compile_rel_App_Lam \\ fs []
+    \\ irule_at Any state_app_unit_2ProofTheory.compile_rel_App \\ fs []
+    \\ once_rewrite_tac [state_app_unit_2ProofTheory.compile_rel_cases] \\ simp []
+    \\ first_x_assum $ irule_at Any \\ fs [])
+  >-
+   (irule_at Any state_app_unit_2ProofTheory.compile_rel_App_Let \\ fs []
+    \\ first_x_assum $ irule_at $ Pos hd \\ fs []
+    \\ first_x_assum $ irule_at $ Pos hd \\ fs []
+    \\ irule_at Any state_app_unit_1ProofTheory.compile_rel_Let \\ fs []
+    \\ irule_at Any state_app_unit_1ProofTheory.compile_rel_App \\ fs []
+    \\ irule_at Any state_app_unit_1ProofTheory.compile_rel_App \\ fs []
+    \\ irule_at Any state_app_unit_1ProofTheory.compile_rel_Let_Var \\ fs []
+    \\ irule_at Any state_app_unit_1ProofTheory.compile_rel_App_Lam \\ fs [])
+  >-
+   (irule_at Any state_app_unit_2ProofTheory.compile_rel_App_If \\ fs []
+    \\ rpt (first_x_assum $ irule_at $ Pos hd \\ fs [])
+    \\ irule_at Any state_app_unit_1ProofTheory.compile_rel_If \\ fs []
+    \\ irule_at Any state_app_unit_1ProofTheory.compile_rel_Let_Var \\ fs []
+    \\ irule_at Any state_app_unit_1ProofTheory.compile_rel_App_Lam \\ fs []
+    \\ rpt (irule_at Any state_app_unit_1ProofTheory.compile_rel_App \\ fs []))
+  >-
+   (irule_at Any state_app_unit_2ProofTheory.compile_rel_App_Letrec \\ fs []
+    \\ rpt (first_x_assum $ irule_at $ Pos hd \\ fs [])
+    \\ irule_at Any state_app_unit_1ProofTheory.compile_rel_Letrec \\ fs []
+    \\ fs [MAP_MAP_o,combinTheory.o_DEF,UNCURRY,EVERY_MAP]
+    \\ rpt (irule_at Any state_app_unit_1ProofTheory.compile_rel_App \\ fs [])
+    \\ drule_all LIST_REL_rel2_rel1
+    \\ strip_tac
+    \\ qexists_tac ‘MAP2 (λ(n,v,_) y. (n,Lam (SOME v) y)) sfns ys’
+    \\ imp_res_tac LIST_REL_LENGTH \\ fs []
+    \\ rpt (pop_assum mp_tac)
+    \\ qid_spec_tac ‘tfns’
+    \\ qid_spec_tac ‘sfns’
+    \\ qid_spec_tac ‘ys’
+    \\ Induct \\ Cases_on ‘sfns’ \\ Cases_on ‘tfns’ \\ fs []
+    \\ PairCases_on ‘h’ \\ PairCases_on ‘h'’ \\ fs []
+    \\ strip_tac \\ rpt $ disch_then assume_tac \\ fs []
+    \\ once_rewrite_tac [state_app_unit_2ProofTheory.compile_rel_cases] \\ simp []
+    \\ once_rewrite_tac [state_app_unit_1ProofTheory.compile_rel_cases] \\ simp []
+    \\ first_x_assum drule_all \\ fs [])
+  >-
+   (irule_at Any state_app_unit_1ProofTheory.compile_rel_Var \\ fs []
+    \\ irule_at Any state_app_unit_2ProofTheory.compile_rel_Var \\ fs [])
+  >-
+   (qexists_tac ‘(Lam ov y)’
+    \\ once_rewrite_tac [state_app_unit_2ProofTheory.compile_rel_cases] \\ simp []
+    \\ once_rewrite_tac [state_app_unit_1ProofTheory.compile_rel_cases] \\ simp [])
+  >-
+   (irule_at Any state_app_unit_1ProofTheory.compile_rel_Raise \\ fs []
+    \\ irule_at Any state_app_unit_2ProofTheory.compile_rel_Raise \\ fs []
+    \\ rpt (first_x_assum $ irule_at $ Pos hd \\ fs []))
+  >-
+   (irule_at Any state_app_unit_1ProofTheory.compile_rel_Handle \\ fs []
+    \\ irule_at Any state_app_unit_2ProofTheory.compile_rel_Handle \\ fs []
+    \\ rpt (first_x_assum $ irule_at $ Pos hd \\ fs []))
+  >-
+   (irule_at Any state_app_unit_1ProofTheory.compile_rel_HandleApp \\ fs []
+    \\ irule_at Any state_app_unit_2ProofTheory.compile_rel_HandleApp \\ fs []
+    \\ rpt (first_x_assum $ irule_at $ Pos hd \\ fs []))
+  >-
+   (irule_at Any state_app_unit_1ProofTheory.compile_rel_App \\ fs []
+    \\ irule_at Any state_app_unit_2ProofTheory.compile_rel_App \\ fs []
+    \\ rpt (first_x_assum $ irule_at $ Pos hd \\ fs []) \\ cheat)
+  >- cheat
+  >-
+   (irule_at Any state_app_unit_1ProofTheory.compile_rel_Let \\ fs []
+    \\ irule_at Any state_app_unit_2ProofTheory.compile_rel_Let \\ fs []
+    \\ rpt (first_x_assum $ irule_at $ Pos hd \\ fs []))
+  >-
+   (irule_at Any state_app_unit_1ProofTheory.compile_rel_If \\ fs []
+    \\ irule_at Any state_app_unit_2ProofTheory.compile_rel_If \\ fs []
+    \\ rpt (first_x_assum $ irule_at $ Pos hd \\ fs []))
+  \\ cheat
 QED
 
-Theorem env_rel_zip:
-  ∀n x y xs ys.
-    env_rel xs ys ∧ LIST_REL v_rel x y ∧ LENGTH n = LENGTH x ⇒
-    env_rel (REVERSE(ZIP(n,x))++xs) (REVERSE(ZIP(n,y))++ys)
+Theorem cexp1_rel_correct:
+  ∀x y. cexp1_rel x y ⇒ itree_of (exp_of x) = itree_of (exp_of y)
+Proof
+  rw [] \\ drule cexp1_rel_thm \\ rw []
+  \\ imp_res_tac state_app_unit_2ProofTheory.compile_rel_itree_of
+  \\ imp_res_tac state_app_unit_1ProofTheory.compile_rel_itree_of
+  \\ simp []
+QED
+
+Theorem cexp1_rel_refl[simp]:
+  ∀x. cexp1_rel x x
+Proof
+  ho_match_mp_tac exp_of_ind \\ rw []
+  \\ simp [Once cexp1_rel_cases]
+  \\ rpt disj2_tac
+  \\ rpt $ pop_assum mp_tac
+  \\ qid_spec_tac ‘funs’
+  \\ qid_spec_tac ‘rows’
+  \\ qid_spec_tac ‘xs’ \\ fs []
+  \\ Induct \\ fs [FORALL_PROD] \\ metis_tac []
+QED
+
+Triviality cexp1_rel_eq: (* TODO: delete *)
+  x = y ⇒ cexp1_rel x y
+Proof
+  rw [] \\ fs []
+QED
+
+Inductive cexp_rel:
+
+[~refl:]
+  (cexp_rel x x) ∧
+
+[~trans:]
+  (cexp_rel x y ∧ cexp_rel y z ⇒ cexp_rel x z) ∧
+
+[~App_Lam:]
+  (cexp_rel x y ⇒
+   cexp_rel (app (Lam NONE x) Unit) y) ∧
+
+[~App_Lam:]
+  (cexp_rel x y ⇒
+   cexp_rel (app (Lam NONE x) Unit) y) ∧
+
+[~App_Let:]
+  (cexp_rel x x1 ∧ cexp_rel y y1 ⇒
+   cexp_rel (app (Let x_opt x y) Unit)
+             (Let x_opt x1 (app y1 Unit))) ∧
+
+[~App_If:]
+  (cexp_rel x x1 ∧ cexp_rel y y1 ∧ cexp_rel z z1 ⇒
+   cexp_rel (app (If x y z) Unit)
+             (If x1 (app y1 Unit) (app z1 Unit))) ∧
+
+[~App_Letrec:]
+  (cexp_rel y y1 ∧
+   MAP FST tfns = MAP FST sfns ∧
+   MAP (FST o SND) tfns = MAP (FST o SND) sfns ∧
+   LIST_REL cexp_rel (MAP (SND o SND) tfns) (MAP (SND o SND) sfns) ⇒
+   cexp_rel (app (Letrec tfns y) Unit)
+             (Letrec sfns (app y1 Unit))) ∧
+
+[~Var:]
+  cexp_rel (state_cexp$Var v) (state_cexp$Var v) ∧
+
+[~Lam:]
+  (cexp_rel x y ⇒
+  cexp_rel (Lam ov x) (Lam ov y)) ∧
+
+[~Raise:]
+  (cexp_rel x y ⇒
+  cexp_rel (Raise x) (Raise y)) ∧
+
+[~Handle:]
+  (cexp_rel x1 y1 ∧ cexp_rel x2 y2 ⇒
+  cexp_rel (Handle x1 v x2) (Handle y1 v y2)) ∧
+
+[~HandleApp:]
+  (cexp_rel x1 y1 ∧ cexp_rel x2 y2 ⇒
+  cexp_rel (HandleApp x1 x2) (HandleApp y1 y2)) ∧
+
+[~App:]
+  (LIST_REL (cexp_rel) xs ys ⇒
+  cexp_rel (App op xs) (App op ys)) ∧
+
+[~Letrec:]
+  (∀tfns sfns te se.
+    MAP FST tfns = MAP FST sfns ∧
+    MAP (FST o SND) tfns = MAP (FST o SND) sfns ∧
+    LIST_REL cexp_rel (MAP (SND o SND) tfns) (MAP (SND o SND) sfns) ∧
+    cexp_rel te se ⇒
+    cexp_rel (Letrec tfns te) (Letrec sfns se)) ∧
+
+[~Let:]
+  (cexp_rel te1 se1 ∧
+   cexp_rel te2 se2 ⇒
+  cexp_rel (Let x_opt te1 te2) (Let x_opt se1 se2)) ∧
+
+[~If:]
+  (cexp_rel te se ∧
+   cexp_rel te1 se1 ∧
+   cexp_rel te2 se2 ⇒
+  cexp_rel (If te te1 te2) (If se se1 se2)) ∧
+
+[~Case:]
+  (∀v te se tes ses.
+     cexp_rel te se ∧
+     MAP FST tes = MAP FST ses ∧
+     MAP (FST o SND) tes = MAP (FST o SND) ses ∧
+     LIST_REL cexp_rel (MAP (SND o SND) tes) (MAP (SND o SND) ses) ⇒
+  cexp_rel (Case te v tes) (Case se v ses))
+
+End
+
+Triviality NRC_Let:
+  ∀k x x1 y y1.
+    NRC cexp1_rel k x x1 ∧ NRC cexp1_rel k y y1 ⇒
+    NRC cexp1_rel k (Let x_opt x y) (Let x_opt x1 y1)
+Proof
+  Induct \\ fs [NRC,PULL_EXISTS] \\ rw []
+  \\ irule_at Any cexp1_rel_Let
+  \\ rpt $ last_x_assum $ irule_at Any
+QED
+
+Theorem cexp_rel_imp_nrc:
+  ∀x y. cexp_rel x y ⇒ ∃n. NRC cexp1_rel n x y
+Proof
+  Induct_on ‘cexp_rel’ \\ rw []
+  >- (qexists_tac ‘0’ \\ fs [])
+  >- (qexists_tac ‘n+n'’
+      \\ fs [arithmeticTheory.NRC_ADD_EQN]
+      \\ first_assum $ irule_at Any \\ fs [])
+  >-
+   (qexists_tac ‘1+n’
+    \\ rewrite_tac [arithmeticTheory.NRC_ADD_EQN]
+    \\ pop_assum $ irule_at Any
+    \\ fs [] \\ irule cexp1_rel_App_Lam \\ fs [])
+  >-
+   (qexists_tac ‘1+n’
+    \\ rewrite_tac [arithmeticTheory.NRC_ADD_EQN]
+    \\ pop_assum $ irule_at Any
+    \\ fs [] \\ irule cexp1_rel_App_Lam \\ fs [])
+  >-
+   (Q.REFINE_EXISTS_TAC ‘1+k’
+    \\ rewrite_tac [arithmeticTheory.NRC_ADD_EQN] \\ fs []
+    \\ irule_at Any cexp1_rel_App_Let
+    \\ rpt $ irule_at Any cexp1_rel_eq \\ fs []
+    \\ qexists_tac ‘n+n'’
+    \\ irule NRC_Let
+    \\ cheat)
+  >- cheat
+  >-
+   (Q.REFINE_EXISTS_TAC ‘1+k’
+    \\ rewrite_tac [arithmeticTheory.NRC_ADD_EQN] \\ fs []
+    \\ irule_at Any cexp1_rel_App_Letrec
+    \\ cheat)
+  >- (qexists_tac ‘0’ \\ fs [])
+  >- cheat
+  \\ cheat
+QED
+
+Theorem cexp_rel_itree:
+  ∀x y. cexp_rel x y ⇒ itree_of (exp_of x) = itree_of (exp_of y)
+Proof
+  rw []
+  \\ drule cexp_rel_imp_nrc
+  \\ fs [PULL_EXISTS]
+  \\ qid_spec_tac ‘x’
+  \\ qid_spec_tac ‘y’
+  \\ Induct_on ‘n’
+  \\ fs [NRC,PULL_EXISTS]
+  \\ rw [] \\ res_tac
+  \\ imp_res_tac cexp1_rel_correct \\ fs []
+QED
+
+Definition unit_apps_def:
+  unit_apps k x = if k = 0n then (x:cexp) else unit_apps (k-1) (app x Unit)
+End
+
+Theorem unit_apps_0[simp]:
+  unit_apps 0 x = x
+Proof
+  EVAL_TAC
+QED
+
+Definition push_app_unit_def:
+  push_app_unit l ((Var v):cexp) =
+    unit_apps l (Var v) ∧
+  push_app_unit l (App op xs) =
+    (if op = AppOp ∧ LENGTH xs = 2 then
+       if EL 1 xs = Unit then
+         push_app_unit (l+1n) (EL 0 xs)
+       else unit_apps l $ App op (MAP (push_app_unit 0) xs)
+     else unit_apps l $ App op (MAP (push_app_unit 0) xs)) ∧
+  push_app_unit l (Lam vn x) =
+    (if l ≠ 0 ∧ vn = NONE then
+       push_app_unit (l-1n) x
+     else unit_apps l  (Lam vn (push_app_unit 0 x))) ∧
+  push_app_unit l (Letrec funs x) =
+    Letrec (MAP (λ(f,v,y). (f,v,push_app_unit 0 y)) funs) (push_app_unit l x) ∧
+  push_app_unit l (Let vn x y) =
+    Let vn (push_app_unit 0 x) (push_app_unit l y) ∧
+  push_app_unit l (If x y z) =
+    If (push_app_unit 0 x) (push_app_unit l y) (push_app_unit l z) ∧
+  push_app_unit l (Case x v rows) =
+    unit_apps l
+      (Case (push_app_unit 0 x) v (MAP (λ(v,vs,y). (v,vs,push_app_unit 0 y)) rows)) ∧
+  push_app_unit l (Raise x) =
+    unit_apps l (Raise (push_app_unit 0 x)) ∧
+  push_app_unit l (Handle x v y) =
+    unit_apps l (Handle (push_app_unit 0 x) v (push_app_unit 0 y)) ∧
+  push_app_unit l (HandleApp x y) =
+    unit_apps l (HandleApp (push_app_unit 0 x) (push_app_unit 0 y))
+Termination
+  WF_REL_TAC ‘measure (cexp_size o SND)’
+  \\ gvs [LENGTH_EQ_NUM_compute,PULL_EXISTS,cexp_size_eq,list_size_def]
+End
+
+Theorem cexp_rel_unit_apps:
+  ∀l x y. cexp_rel x y ⇒ cexp_rel (unit_apps l x) (unit_apps l y)
 Proof
   Induct \\ fs []
-  \\ Cases_on ‘x’ \\ fs [PULL_EXISTS] \\ rw []
-  \\ full_simp_tac std_ss [GSYM APPEND_ASSOC,APPEND]
-  \\ last_x_assum irule \\ fs []
-  \\ irule env_rel_cons \\ fs []
+  \\ once_rewrite_tac [unit_apps_def] \\ fs []
+  \\ rw [] \\ first_x_assum irule
+  \\ irule cexp_rel_App
+  \\ fs [cexp_rel_refl]
 QED
 
-Triviality FST_INTRO:
-  (λ(p1,p2). p1) = FST
+Theorem cexp_rel_pust_app_unit:
+  ∀l x. cexp_rel (unit_apps l x) (push_app_unit l x)
 Proof
-  fs [FUN_EQ_THM,FORALL_PROD]
-QED
-
-Theorem ALOOKUP_rec:
-  ALOOKUP (MAP (λ(fn,_). (fn,g fn)) tfns) n = SOME tv <=>
-  MEM n (MAP FST tfns) ∧ tv = g n
-Proof
-  Induct_on ‘tfns’ \\ fs [FORALL_PROD]
-  \\ rw [] \\ eq_tac \\ rw []
-QED
-
-Theorem ALOOKUP_list_rel:
-  ∀tfns sfns n x.
-    ALOOKUP tfns n = SOME x ∧
-    LIST_REL (compile_rel 0) (MAP SND tfns) (MAP SND sfns) ∧
-    MAP FST tfns = MAP FST sfns ⇒
-    ∃y. ALOOKUP sfns n = SOME y ∧ compile_rel 0 x y
-Proof
-  Induct \\ fs [FORALL_PROD,PULL_EXISTS] \\ rw []
-  \\ Cases_on‘sfns’ \\ gvs [] \\ PairCases_on ‘h’ \\ fs []
-QED
-
-Theorem get_atoms_thm:
-  ∀tvs svs. LIST_REL v_rel tvs svs ⇒ get_atoms tvs = get_atoms svs
-Proof
-  Induct \\ fs [PULL_EXISTS]
-  \\ simp [Once v_rel_cases]
-  \\ rw [] \\ fs [get_atoms_def]
-  \\ res_tac \\ fs []
-QED
-
-Theorem application_thm:
-  application op tenv tvs ts tk = (tr1,ts1,tk1) ∧
-  OPTREL (LIST_REL (LIST_REL v_rel)) ts ss ∧ cont_rel 0 tk sk ∧
-  LIST_REL v_rel tvs svs ∧ env_rel tenv senv ∧
-  num_args_ok op (LENGTH svs) ⇒
-  ∃sr1 ss1 sk1.
-    application op senv svs ss sk = (sr1,ss1,sk1) ∧
-    OPTREL (LIST_REL (LIST_REL v_rel)) ts1 ss1 ∧
-    step_res_rel tr1 tk1 sr1 sk1
-Proof
-  Cases_on ‘op’ \\ fs [num_args_ok_def,LENGTH_EQ_NUM_compute,PULL_EXISTS]
-  \\ rw [] \\ gvs []
-  >~ [‘Cons’] >-
-   (gvs [application_def,step,step_res_rel_cases]
-    \\ simp [Once v_rel_cases])
-  >~ [‘Proj’] >-
-   (gvs [application_def,step,AllCaseEqs()]
-    \\ qpat_x_assum ‘v_rel _ _’ mp_tac
-    \\ simp [Once v_rel_cases] \\ strip_tac \\ gvs [step_res_rel_cases]
-    \\ imp_res_tac LIST_REL_LENGTH \\ gvs []
-    \\ gvs [LIST_REL_EL_EQN])
-  >~ [‘IsEq’] >-
-   (gvs [application_def,step,AllCaseEqs()]
-    \\ qpat_x_assum ‘v_rel _ _’ mp_tac
-    \\ simp [Once v_rel_cases] \\ strip_tac \\ gvs [step_res_rel_cases]
-    \\ imp_res_tac LIST_REL_LENGTH \\ gvs [] \\ rw []
-    \\ simp [Once v_rel_cases] \\ strip_tac \\ gvs [step_res_rel_cases])
-  >~ [‘AppOp’] >-
-   (gvs [application_def]
-    \\ qpat_x_assum ‘v_rel x h’ mp_tac
-    \\ simp [Once v_rel_cases]
-    \\ strip_tac \\ gvs [dest_anyClosure_def,dest_Closure_def,step,step_res_rel_cases]
+  ho_match_mp_tac push_app_unit_ind \\ rpt strip_tac
+  >- fs [push_app_unit_def,cexp_rel_refl]
+  >-
+   (reverse (Cases_on ‘op = AppOp ∧ LENGTH xs = 2 ∧ EL 1 xs = Unit’ \\ gvs [])
+    \\ gvs [push_app_unit_def]
     >-
-     (rpt $ first_assum $ irule_at Any
-      \\ Cases_on ‘n’ \\ gvs [opt_bind_def]
-      \\ irule env_rel_cons \\ fs [])
-    \\ gvs [AllCaseEqs(),ALOOKUP_NONE]
-    \\ drule ALOOKUP_MEM \\ strip_tac
-    \\ fs [EVERY_MEM,FORALL_PROD]
-    \\ first_assum drule \\ simp_tac (srw_ss()) []
-    \\ drule_all ALOOKUP_list_rel
-    \\ strip_tac \\ fs []
+     (rw [] \\ gvs []
+      \\ irule cexp_rel_unit_apps
+      \\ irule cexp_rel_App
+      \\ qpat_x_assum ‘∀x. _’ mp_tac
+      \\ qid_spec_tac ‘xs’ \\ Induct \\ fs []
+      \\ metis_tac [])
+    \\ gvs [LENGTH_EQ_NUM_compute]
     \\ pop_assum mp_tac
-    \\ simp [Once compile_rel_cases]
-    \\ strip_tac \\ fs []
-    \\ ‘MEM n (MAP FST sfns)’ by
-     (imp_res_tac ALOOKUP_MEM \\ fs [MEM_MAP,EXISTS_PROD]
-      \\ first_assum $ irule_at Any) \\ fs []
-    \\ rpt $ first_assum $ irule_at Any
-    \\ Cases_on ‘arg’ \\ fs []
-    \\ gvs [opt_bind_def]
-    \\ TRY (irule env_rel_cons) \\ fs []
-    \\ gvs [env_rel_def,ALOOKUP_APPEND,AllCaseEqs(),ALOOKUP_NONE]
-    \\ gvs [MAP_MAP_o,combinTheory.o_DEF,LAMBDA_PROD,FST_INTRO,ALOOKUP_rec]
-    \\ strip_tac \\ Cases_on ‘MEM n' (MAP FST sfns)’ \\ fs []
-    \\ rw [Once v_rel_cases] \\ fs [env_rel_def]
-    \\ fs [EVERY_MEM,FORALL_PROD,LAMBDA_PROD]
-    \\ rw [] \\ res_tac \\ fs [])
-  >~ [‘Alloc’] >-
-   (gvs [application_def,step,step_res_rel_cases]
-    \\ qpat_x_assum ‘v_rel x h’ mp_tac
-    \\ simp [Once v_rel_cases] \\ strip_tac \\ gvs []
-    \\ gvs [AllCaseEqs()]
-    \\ Cases_on ‘ss’ \\ gvs []
-    \\ imp_res_tac LIST_REL_LENGTH \\ fs []
-    \\ simp [Once v_rel_cases]
-    \\ fs [LIST_REL_SNOC]
-    \\ simp [LIST_REL_EL_EQN,EL_REPLICATE])
-  >~ [‘Ref’] >-
-   (gvs [application_def,step,step_res_rel_cases]
-    \\ Cases_on ‘ts’ \\ Cases_on ‘ss’ \\ gvs []
-    \\ imp_res_tac LIST_REL_LENGTH \\ fs []
-    \\ simp [Once v_rel_cases]
-    \\ fs [LIST_REL_SNOC])
-  >~ [‘Length’] >-
-   (gvs [application_def,step,step_res_rel_cases]
-    \\ qpat_x_assum ‘v_rel x h’ mp_tac
-    \\ simp [Once v_rel_cases] \\ strip_tac \\ gvs []
-    \\ Cases_on ‘a’ \\ gvs []
-    \\ Cases_on ‘ts’ \\ Cases_on ‘ss’ \\ gvs []
-    \\ imp_res_tac LIST_REL_LENGTH \\ fs [oEL_THM]
-    \\ IF_CASES_TAC \\ gvs []
-    \\ simp [Once v_rel_cases]
-    \\ gvs [LIST_REL_EL_EQN])
-  >~ [‘Sub’] >-
-   (gvs [application_def,step,step_res_rel_cases]
-    \\ qpat_x_assum ‘v_rel x h’ mp_tac
-    \\ simp [Once v_rel_cases] \\ strip_tac \\ gvs []
-    \\ Cases_on ‘a’ \\ gvs []
-    \\ qpat_x_assum ‘v_rel _ _’ mp_tac
-    \\ simp [Once v_rel_cases] \\ strip_tac \\ gvs []
-    \\ Cases_on ‘a’ \\ gvs []
-    \\ Cases_on ‘ts’ \\ Cases_on ‘ss’ \\ gvs []
-    \\ imp_res_tac LIST_REL_LENGTH \\ fs [oEL_THM]
-    \\ rpt (IF_CASES_TAC \\ gvs [])
-    \\ gvs [LIST_REL_EL_EQN]
-    \\ ntac 2 (simp [Once compile_rel_cases,env_rel_def])
-    \\ imp_res_tac integerTheory.NUM_POSINT_EXISTS \\ gvs []
-    \\ simp[Once v_rel_cases]
-    \\ rpt $ first_assum $ irule_at Any)
-  >~ [‘UnsafeSub’] >-
-   (gvs [application_def,step,step_res_rel_cases]
-    \\ qpat_x_assum ‘v_rel x h’ mp_tac
-    \\ simp [Once v_rel_cases] \\ strip_tac \\ gvs []
-    \\ Cases_on ‘a’ \\ gvs []
-    \\ qpat_x_assum ‘v_rel _ _’ mp_tac
-    \\ simp [Once v_rel_cases] \\ strip_tac \\ gvs []
-    \\ Cases_on ‘a’ \\ gvs []
-    \\ Cases_on ‘ts’ \\ Cases_on ‘ss’ \\ gvs []
-    \\ imp_res_tac LIST_REL_LENGTH \\ fs [oEL_THM]
-    \\ rpt (IF_CASES_TAC \\ gvs [])
-    \\ gvs [LIST_REL_EL_EQN]
-    \\ ntac 2 (simp [Once compile_rel_cases,env_rel_def])
-    \\ imp_res_tac integerTheory.NUM_POSINT_EXISTS \\ gvs [])
-  >~ [‘Update’] >-
-   (gvs [application_def,step,step_res_rel_cases]
-    \\ qpat_x_assum ‘v_rel x h’ mp_tac
-    \\ simp [Once v_rel_cases] \\ strip_tac \\ gvs []
-    \\ Cases_on ‘a’ \\ gvs []
-    \\ qpat_x_assum ‘v_rel _ h'’ mp_tac
-    \\ simp [Once v_rel_cases] \\ strip_tac \\ gvs []
-    \\ Cases_on ‘a’ \\ gvs []
-    \\ Cases_on ‘ts’ \\ Cases_on ‘ss’ \\ gvs []
-    \\ imp_res_tac LIST_REL_LENGTH \\ fs [oEL_THM]
-    \\ rpt (IF_CASES_TAC \\ gvs [])
-    \\ gvs [LIST_REL_EL_EQN]
-    \\ ntac 2 (simp [Once compile_rel_cases,env_rel_def])
-    \\ imp_res_tac integerTheory.NUM_POSINT_EXISTS \\ gvs []
-    \\ gvs [EL_LUPDATE] \\ rw []
-    \\ gvs [EL_LUPDATE] \\ rw []
-    \\ simp [Once v_rel_cases] \\ rpt strip_tac \\ gvs []
-    \\ rpt $ first_assum $ irule_at Any)
-  >~ [‘UnsafeUpdate’] >-
-   (gvs [application_def,step,step_res_rel_cases]
-    \\ qpat_x_assum ‘v_rel x h’ mp_tac
-    \\ simp [Once v_rel_cases] \\ strip_tac \\ gvs []
-    \\ Cases_on ‘a’ \\ gvs []
-    \\ qpat_x_assum ‘v_rel _ h'’ mp_tac
-    \\ simp [Once v_rel_cases] \\ strip_tac \\ gvs []
-    \\ Cases_on ‘a’ \\ gvs []
-    \\ Cases_on ‘ts’ \\ Cases_on ‘ss’ \\ gvs []
-    \\ imp_res_tac LIST_REL_LENGTH \\ fs [oEL_THM]
-    \\ rpt (IF_CASES_TAC \\ gvs [])
-    \\ gvs [LIST_REL_EL_EQN]
-    \\ ntac 2 (simp [Once compile_rel_cases,env_rel_def])
-    \\ imp_res_tac integerTheory.NUM_POSINT_EXISTS \\ gvs []
-    \\ gvs [EL_LUPDATE] \\ rw []
-    \\ gvs [EL_LUPDATE] \\ rw []
-    \\ simp [Once v_rel_cases] \\ strip_tac \\ gvs [])
-  >~ [‘FFI’] >-
-   (gvs [application_def,step,step_res_rel_cases]
-    \\ qpat_x_assum ‘v_rel x h’ mp_tac
-    \\ simp [Once v_rel_cases] \\ strip_tac \\ gvs []
-    \\ Cases_on ‘a’ \\ gvs []
-    \\ Cases_on ‘ts’ \\ Cases_on ‘ss’ \\ gvs [])
-  \\ rename [‘AtomOp’]
-  \\ gvs [application_def,step,step_res_rel_cases]
-  \\ imp_res_tac get_atoms_thm \\ gvs [AllCaseEqs()]
-  \\ simp [Once v_rel_cases]
-QED
-
-Theorem step_1_Exp_forward:
-  ∀n e1 e2 ts tk sr1 ss1 sk1 ss sk env1 env2.
-    step ss sk (Exp env2 e2) = (sr1,ss1,sk1) ∧
-    cont_rel n tk sk ∧
-    OPTREL (LIST_REL (LIST_REL v_rel)) ts ss ∧
-    compile_rel n e1 e2 ∧
-    env_rel env1 env2 ⇒
-    ∃m tr1 ts1 tk1.
-      step_n (m + 1) (Exp env1 e1,ts,tk) = (tr1,ts1,tk1) ∧
-      (tr1 ≠ Error ⇒
-       OPTREL (LIST_REL (LIST_REL v_rel)) ts1 ss1 ∧
-       step_res_rel tr1 tk1 sr1 sk1)
-Proof
-  Induct_on ‘compile_rel’ \\ rpt strip_tac
+    \\ simp [Once unit_apps_def])
   >-
-   (fs [GSYM ADD1]
-    \\ Q.REFINE_EXISTS_TAC ‘SUC ck’ \\ simp [ADD_CLAUSES,step_n_SUC,step]
-    \\ Q.REFINE_EXISTS_TAC ‘SUC ck’ \\ simp [ADD_CLAUSES,step_n_SUC,step]
-    \\ Q.REFINE_EXISTS_TAC ‘SUC ck’
-    \\ first_x_assum irule
-    \\ rpt (first_assum $ irule_at $ Pos hd \\ fs [])
-    \\ fs [ADD1]
-    \\ simp [Once cont_rel_cases])
-  >-
-   (qpat_x_assum ‘cont_rel (n + 1) tk sk’ mp_tac
-    \\ simp [Once cont_rel_cases] \\ strip_tac \\ gvs []
-    \\ fs [GSYM ADD1] \\ simp [ADD_CLAUSES,step_n_SUC,step]
-    \\ Q.REFINE_EXISTS_TAC ‘SUC ck’ \\ simp [ADD_CLAUSES,step_n_SUC,step]
-    \\ Q.REFINE_EXISTS_TAC ‘SUC ck’ \\ simp [ADD_CLAUSES,step_n_SUC,step]
-    \\ first_x_assum drule_all \\ strip_tac
-    \\ fs [ADD_CLAUSES,step_n_SUC,step]
-    \\ first_x_assum $ irule_at Any \\ gvs [])
-  \\ gvs []
-  \\ rpt (qpat_x_assum ‘∀x. _’ kall_tac)
-  >~ [‘Var v’] >-
-   (qexists_tac ‘0’ \\ gvs [step]
-    \\ Cases_on ‘ALOOKUP env1 v’ \\ gvs []
-    \\ gvs [env_rel_def]
-    \\ res_tac \\ gvs []
-    \\ gvs [step_res_rel_cases,env_rel_def])
-  >~ [‘If’] >-
-   (qexists_tac ‘0’ \\ gvs [step]
-    \\ fs [step_res_rel_cases]
-    \\ last_x_assum $ irule_at Any \\ fs []
-    \\ simp [Once cont_rel_cases]
-    \\ rpt (last_x_assum $ irule_at Any \\ fs []))
-  >~ [‘Lam’] >-
-   (qexists_tac ‘0’ \\ fs []
-    \\ gvs [step,AllCaseEqs(),env_rel_def,step_res_rel_cases]
-    \\ once_rewrite_tac [Once v_rel_cases] \\ fs [env_rel_def])
-  >~ [‘Raise’] >-
-   (qexists_tac ‘0’ \\ fs []
-    \\ gvs [step,AllCaseEqs(),env_rel_def,step_res_rel_cases]
-    \\ once_rewrite_tac [Once v_rel_cases] \\ fs [env_rel_def]
-    \\ last_x_assum $ irule_at Any \\ fs []
-    \\ simp [Once cont_rel_cases]
-    \\ last_x_assum $ irule_at Any \\ fs [])
-  >~ [‘Letrec’] >-
-   (qexists_tac ‘0’ \\ fs [step]
-    \\ simp [step,AllCaseEqs(),env_rel_def,step_res_rel_cases]
-    \\ rpt $ first_x_assum $ irule_at Any \\ gvs []
-    \\ rpt gen_tac
-    \\ gvs [env_rel_def,ALOOKUP_APPEND,AllCaseEqs(),ALOOKUP_NONE]
-    \\ gvs [MAP_MAP_o,combinTheory.o_DEF,LAMBDA_PROD,FST_INTRO,ALOOKUP_rec]
-    \\ strip_tac \\ Cases_on ‘MEM n' (MAP FST sfns)’ \\ fs []
-    \\ rw [Once v_rel_cases] \\ fs [env_rel_def]
-    \\ first_x_assum (fn th => mp_tac th \\ match_mp_tac LIST_REL_mono)
-    \\ fs [])
-  >~ [‘Let’] >-
-   (qexists_tac ‘0’ \\ gvs [step]
-    \\ simp [step,AllCaseEqs(),step_res_rel_cases]
-    \\ rpt $ first_x_assum $ irule_at Any \\ gvs []
-    \\ simp [Once cont_rel_cases]
-    \\ rpt $ first_x_assum $ irule_at Any \\ gvs [])
-  >~ [‘Handle’] >-
-   (qexists_tac ‘0’ \\ gvs [step]
-    \\ simp [step,AllCaseEqs(),step_res_rel_cases]
-    \\ rpt $ first_x_assum $ irule_at Any \\ gvs []
-    \\ simp [Once cont_rel_cases])
-  >~ [‘HandleApp’] >-
-   (qexists_tac ‘0’ \\ gvs [step]
-    \\ simp [step,AllCaseEqs(),step_res_rel_cases]
-    \\ rpt $ first_x_assum $ irule_at Any \\ gvs []
-    \\ simp [Once cont_rel_cases])
-  >~ [‘Case’] >-
-   (qexists_tac ‘0’ \\ gvs [step]
-    \\ IF_CASES_TAC \\ gvs []
-    \\ simp [step,AllCaseEqs(),step_res_rel_cases]
-    \\ rpt $ first_x_assum $ irule_at Any \\ gvs []
-    \\ simp [Once cont_rel_cases]
-    \\ rpt $ first_x_assum $ irule_at Any \\ gvs []
-    \\ first_x_assum (fn th => mp_tac th \\ match_mp_tac LIST_REL_mono)
-    \\ fs [])
-  >~ [‘App’] >-
-   (qexists_tac ‘0’ \\ gvs [step]
-    \\ IF_CASES_TAC \\ gvs []
-    \\ imp_res_tac LIST_REL_LENGTH \\ fs []
-    \\ gvs [AllCaseEqs()]
-    >-
-     (‘∃a. application op env1 [] ts tk = a’ by fs [] \\ PairCases_on ‘a’
-      \\ drule application_thm \\ fs []
-      \\ disch_then drule_all \\ strip_tac \\ gvs [])
-    \\ gvs [SWAP_REVERSE_SYM]
-    \\ Cases_on ‘xs’ using SNOC_CASES \\ fs [PULL_EXISTS]
-    \\ gvs [GSYM SWAP_REVERSE_SYM]
-    \\ full_simp_tac std_ss [GSYM SNOC_APPEND,LIST_REL_SNOC]
-    \\ gvs []
-    \\ simp [step,AllCaseEqs(),step_res_rel_cases]
-    \\ rpt $ first_x_assum $ irule_at Any \\ gvs []
-    \\ simp [Once cont_rel_cases]
-    \\ drule EVERY2_REVERSE \\ simp_tac std_ss [REVERSE_REVERSE]
-    \\ match_mp_tac LIST_REL_mono \\ fs [])
+   (Cases_on ‘l = 0’ \\ gvs [push_app_unit_def]
+    >- (irule cexp_rel_Lam \\ fs [])
+    \\ reverse (Cases_on ‘vn’) \\ fs []
+    >- (irule cexp_rel_unit_apps \\ irule cexp_rel_Lam \\ fs [])
+    \\ irule cexp_rel_trans
+    \\ first_x_assum $ irule_at Any
+    \\ simp [Once unit_apps_def]
+    \\ irule cexp_rel_unit_apps
+    \\ irule cexp_rel_App_Lam \\ fs [cexp_rel_refl])
+  \\ cheat
 QED
 
-Theorem cont_rel_Exn:
-  ∀n tk sk.
-    cont_rel n tk sk ⇒
-    ∃tk1. step_n n (Exn v,ts,tk) = (Exn v,ts,tk1) ∧ cont_rel 0 tk1 sk
+Theorem itree_of_push_app_unit:
+  itree_of (exp_of (push_app_unit 0 x)) = itree_of (exp_of x)
 Proof
-  Induct \\ fs [step]
-  \\ simp [Once cont_rel_cases,ADD1]
-  \\ rw [] \\ fs [step,step_n_add]
-  \\ last_x_assum irule
-  \\ first_assum $ irule_at Any
+  once_rewrite_tac [EQ_SYM_EQ]
+  \\ simp_tac std_ss [Once $ GSYM unit_apps_0]
+  \\ irule cexp_rel_itree
+  \\ fs [cexp_rel_pust_app_unit]
 QED
 
-Theorem step_1_forward:
-  ∀tr ts tk sr1 ss1 sk1 ss sr sk.
-    step_n 1 (sr,ss,sk) = (sr1,ss1,sk1) ∧
-    OPTREL (LIST_REL (LIST_REL v_rel)) ts ss ∧
-    step_res_rel tr tk sr sk ⇒
-    ∃m tr1 ts1 tk1.
-      step_n (m+1) (tr,ts,tk) = (tr1,ts1,tk1) ∧
-      (tr1 ≠ Error ⇒
-       OPTREL (LIST_REL (LIST_REL v_rel)) ts1 ss1 ∧
-       step_res_rel tr1 tk1 sr1 sk1)
+Triviality push_app_unit_test:
+  push_app_unit 0 (App AppOp [Let NONE (Var w) (Lam NONE (Var v)); Unit]) =
+  Let NONE (Var w) (Var v)
 Proof
-  rpt strip_tac
-  \\ Cases_on ‘is_halt (tr,ts,tk)’
-  >-
-   (‘is_halt (sr,ss,sk)’ by
-        (gvs [step_res_rel_cases] \\ gvs [Once cont_rel_cases])
-    \\ full_simp_tac std_ss [is_halt_step] \\ gvs [])
-  \\ qpat_x_assum ‘step_res_rel tr tk sr sk’ mp_tac
-  \\ simp [Once step_res_rel_cases]
-  \\ strip_tac \\ gvs []
-  >~ [‘Exp’] >-
-   (irule step_1_Exp_forward
-    \\ rpt $ first_assum $ irule_at Any \\ fs [])
-  >~ [‘Exn’] >-
-   (Cases_on ‘tk’ \\ gvs []
-    \\ Cases_on ‘sk’ \\ gvs []
-    >- fs [Once cont_rel_cases]
-    \\ rename [‘cont_rel _ (tk1::tk) (sk1::sk)’]
-    \\ qpat_x_assum ‘cont_rel _ _ _’ mp_tac
-    \\ simp [Once cont_rel_cases]
-    \\ rw [] \\ fs [step] \\ gvs []
-    \\ TRY (qexists_tac ‘0’ \\ fs [step,step_res_rel_cases]
-            \\ irule env_rel_cons \\ fs []
-            \\ first_assum $ irule_at $ Pos last \\ fs [] \\ NO_TAC)
-    \\ TRY
-     (rename [‘cont_rel n’]
-      \\ qexists_tac ‘n’ \\ fs [step_n_add,step]
-      \\ drule cont_rel_Exn
-      \\ disch_then $ qspecl_then [‘v1’,‘ts’] mp_tac
-      \\ strip_tac \\ first_assum $ irule_at Any
-      \\ fs [step_res_rel_cases] \\ NO_TAC)
-    >~ [‘HandleK’] >-
-     (qexists_tac ‘0’ \\ simp [ADD_CLAUSES,step_n_SUC,step]
-      \\ fs [step_res_rel_cases]
-      \\ first_x_assum $ irule_at Any \\ fs []
-      \\ irule_at Any env_rel_cons \\ fs [])
-    \\ rename [‘HandleAppK’]
-    \\ qexists_tac ‘0’ \\ simp [ADD_CLAUSES,step_n_SUC,step]
-    \\ fs [step_res_rel_cases]
-    \\ first_x_assum $ irule_at Any \\ fs []
-    \\ simp [Once cont_rel_cases])
-  \\ qexists_tac ‘0’
-  \\ Cases_on ‘tk’ \\ fs []
-  \\ Cases_on ‘sk’ \\ fs []
-  >- fs [Once cont_rel_cases]
-  \\ rename [‘cont_rel _ (tk1::tk) (sk1::sk)’]
-  \\ qpat_x_assum ‘cont_rel _ _ _’ mp_tac
-  \\ simp [Once cont_rel_cases] \\ rw []
-  >~ [‘IfK’] >-
-   (gvs [step]
-    \\ Cases_on ‘v1 = Constructor "True" [] ∨ v1 = Constructor "False" []’ \\ gvs []
-    \\ gvs [step]
-    \\ qpat_x_assum ‘v_rel _ _’ mp_tac
-    \\ simp [Once v_rel_cases] \\ rw []
-    \\ fs [step_res_rel_cases]
-    \\ first_assum $ irule_at Any \\ fs [])
-  >~ [‘RaiseK’] >-
-   (gvs [step] \\ fs [step_res_rel_cases]
-    \\ Cases_on ‘ts’ \\ Cases_on ‘ss’ \\ gvs [])
-  >~ [‘HandleK’] >-
-   (gvs [step] \\ fs [step_res_rel_cases])
-  >~ [‘HandleAppK’] >-
-   (gvs [step] \\ fs [step_res_rel_cases])
-  >~ [‘LetK _ n’] >-
-   (Cases_on ‘n’ \\ gvs [step,step_res_rel_cases]
-    \\ first_assum $ irule_at Any \\ fs []
-    \\ irule env_rel_cons \\ simp [])
-  >~ [‘CaseK _ v’] >-
-   (Cases_on ‘tes’ \\ gvs [step,return_def]
-    \\ PairCases_on ‘h’ \\ fs [step]
-    \\ Cases_on ‘ses’ \\ gvs []
-    \\ PairCases_on ‘h’ \\ fs [step]
-    \\ IF_CASES_TAC >- fs []
-    \\ CASE_TAC \\ fs []
-    \\ qpat_x_assum ‘v_rel (Constructor _ _) _’ mp_tac
-    \\ simp [Once v_rel_cases] \\ strip_tac \\ gvs []
-    \\ gvs [AllCaseEqs()]
-    >-
-     (fs [step_res_rel_cases,PULL_EXISTS]
-      \\ imp_res_tac LIST_REL_LENGTH \\ fs []
-      \\ first_assum $ irule_at Any \\ fs []
-      \\ rewrite_tac [GSYM APPEND_ASSOC,APPEND]
-      \\ irule env_rel_zip \\ fs []
-      \\ irule_at Any env_rel_cons
-      \\ first_assum $ irule_at $ Pos hd
-      \\ simp [Once v_rel_cases])
-    \\ fs [step_res_rel_cases,PULL_EXISTS]
-    \\ imp_res_tac LIST_REL_LENGTH \\ fs []
-    \\ simp [Once v_rel_cases]
-    \\ simp [Once cont_rel_cases]
-    \\ first_assum $ irule_at $ Pos hd
-    \\ fs [])
-  \\ rename [‘AppK’]
-  \\ reverse (Cases_on ‘tes’) \\ gvs [] \\ gvs [step]
-  >-
-   (simp [Once cont_rel_cases, step_res_rel_cases] \\ rw []
-    \\ first_assum $ irule_at Any \\ fs []
-    \\ simp [Once cont_rel_cases])
-  \\ imp_res_tac LIST_REL_LENGTH \\ gvs []
-  \\ IF_CASES_TAC \\ gs[]
-  \\ ‘∃x. application op tenv (v1::tvs) ts tk = x’ by fs []
-  \\ PairCases_on ‘x’
-  \\ drule application_thm \\ fs [PULL_EXISTS]
-  \\ disch_then drule_all \\ strip_tac \\ gvs []
-QED
-
-Theorem step_n_forward:
-  ∀n tr ts tk sr1 ss1 sk1 ss sr sk.
-    step_n n (sr,ss,sk) = (sr1,ss1,sk1) ∧
-    OPTREL (LIST_REL (LIST_REL v_rel)) ts ss ∧
-    step_res_rel tr tk sr sk ⇒
-    ∃m tr1 ts1 tk1.
-      step_n (m+n) (tr,ts,tk) = (tr1,ts1,tk1) ∧
-      (tr1 ≠ Error ⇒ OPTREL (LIST_REL (LIST_REL v_rel)) ts1 ss1 ∧
-                     step_res_rel tr1 tk1 sr1 sk1)
-Proof
-  Induct \\ fs [] \\ rw []
-  >- (qexists_tac ‘0’ \\ fs [])
-  \\ full_simp_tac std_ss [ADD_CLAUSES]
-  \\ ‘∃a. step_n 1 (sr,ss,sk) = a’ by fs []
-  \\ PairCases_on ‘a’
-  \\ drule_all step_1_forward
-  \\ strip_tac \\ fs []
-  \\ Cases_on ‘tr1 = Error’
-  >-
-   (rewrite_tac [Once ADD_COMM]
-    \\ rewrite_tac [ADD1]
-    \\ rewrite_tac [GSYM ADD_ASSOC]
-    \\ qexists_tac ‘m’
-    \\ once_rewrite_tac [step_n_add]
-    \\ fs [] \\ gvs [is_halt_step,is_halt_def])
-  \\ gvs [step_n_SUC,GSYM ADD1]
-  \\ first_x_assum drule_all
-  \\ strip_tac
-  \\ qexists_tac ‘m+m'’
-  \\ rewrite_tac [GSYM ADD_ASSOC]
-  \\ rewrite_tac [Once ADD_COMM]
-  \\ once_rewrite_tac [step_n_add] \\ fs []
-QED
-
-Theorem cont_rel_nil:
-  (cont_rel 0 [] y ⇔ y = []) ∧
-  (cont_rel 0 x [] ⇔ x = [])
-Proof
-  ntac 2 $ fs [Once cont_rel_cases]
-QED
-
-Theorem step_until_halt_thm:
-  step_res_rel tr tk sr sk ∧
-  OPTREL (LIST_REL (LIST_REL v_rel)) ts ss ∧
-  step_until_halt (tr,ts,tk) ≠ Err ⇒
-  snext_res_rel (step_until_halt (tr,ts,tk))
-                (step_until_halt (sr,ss,sk))
-Proof
-  fs [step_until_halt_def]
-  \\ DEEP_INTRO_TAC some_intro \\ fs [] \\ rw []
-  >-
-   (‘∃a. step_n x (tr,ts,tk) = a’ by fs []
-    \\ PairCases_on ‘a’ \\ gvs []
-    \\ ‘a0 ≠ Error’ by (strip_tac \\ gvs [])
-    \\ reverse (DEEP_INTRO_TAC some_intro \\ fs [] \\ rw [])
-    >-
-     (‘∃b. step_n x (sr,ss,sk) = b’ by fs []
-      \\ PairCases_on ‘b’ \\ gvs []
-      \\ drule_all step_n_forward \\ rw []
-      \\ gvs [step_n_add,is_halt_step]
-      \\ first_x_assum $ qspec_then ‘x’ mp_tac
-      \\ fs []
-      \\ Cases_on ‘a0’ \\ gvs [step_res_rel_cases,cont_rel_nil])
-    \\ ‘∃b. step_n x' (sr,ss,sk) = b’ by fs []
-    \\ PairCases_on ‘b’ \\ gvs []
-    \\ drule_all step_n_forward \\ rw []
-    \\ Cases_on ‘tr1 = Error’
-    >-
-     (‘step_n x (tr,ts,tk) = step_n (m+x') (tr,ts,tk)’
-        by metis_tac [is_halt_imp_eq,is_halt_def] \\ fs [])
-    \\ gs []
-    \\ ‘is_halt (tr1,ts1,tk1)’ by
-     (ntac 5 $ pop_assum mp_tac
-      \\ simp [step_res_rel_cases]
-      \\ rw [] \\ gvs [cont_rel_nil])
-    \\ ‘step_n x (tr,ts,tk) = step_n (m+x') (tr,ts,tk)’
-        by metis_tac [is_halt_imp_eq,is_halt_def] \\ fs []
-    \\ gvs []
-    \\ gvs [step_res_rel_cases]
-    \\ fs [snext_res_rel_cases])
-  \\ reverse (DEEP_INTRO_TAC some_intro \\ fs [] \\ rw [])
-  >- simp [Once snext_res_rel_cases]
-  \\ ‘∃a. step_n x (sr,ss,sk) = a’ by fs []
-  \\ PairCases_on ‘a’ \\ gvs []
-  \\ ‘∃b. step_n x (tr,ts,tk) = b’ by fs []
-  \\ PairCases_on ‘b’ \\ gvs []
-  \\ drule_all step_n_forward \\ rw []
-  \\ last_assum $ qspec_then ‘m+x’ assume_tac
-  \\ last_x_assum $ qspec_then ‘x’ assume_tac
-  \\ gvs []
-  \\ Cases_on ‘tr1 = Error’ \\ gs []
-  \\ gvs [step_res_rel_cases,cont_rel_nil]
-QED
-
-Theorem semantics_thm:
-  compile_rel 0 e1 e2 ∧
-  OPTREL (LIST_REL (LIST_REL v_rel)) ts ss ∧
-  env_rel tenv senv ∧
-  cont_rel 0 tk sk ⇒
-  semantics e1 tenv ts tk --->
-  semantics e2 senv ss sk
-Proof
-  qsuff_tac ‘
-    ∀t1 t2.
-      (∃e1 e2 ts ss tenv senv tk sk.
-        compile_rel 0 e1 e2 ∧
-        OPTREL (LIST_REL (LIST_REL v_rel)) ts ss ∧
-        env_rel tenv senv ∧
-        cont_rel 0 tk sk ∧
-        t1 = semantics e1 tenv ts tk ∧
-        t2 = semantics e2 senv ss sk) ⇒
-      t1 ---> t2’
-  >- (rw [PULL_EXISTS]
-      \\ last_x_assum drule
-      \\ rpt (disch_then drule) \\ fs [])
-  \\ ho_match_mp_tac pure_semanticsTheory.compiles_to_coind
-  \\ rpt gen_tac \\ strip_tac
-  \\ ntac 2 (pop_assum $ mp_tac o GSYM)
-  \\ simp [stateLangTheory.semantics_def]
-  \\ simp [Once sinterp_def] \\ strip_tac
-  \\ simp [Once sinterp_def] \\ strip_tac
-  \\ ntac 2 $ pop_assum mp_tac
-  \\ once_rewrite_tac [itreeTheory.itree_unfold_err]
-  \\ fs []
-  \\ simp [GSYM sinterp_def]
-  \\ Cases_on ‘step_until_halt (Exp tenv e1,ts,tk) = Err’ >- fs []
-  \\ drule_at (Pos last) step_until_halt_thm
-  \\ rpt (disch_then $ drule_at $ Pos last)
-  \\ disch_then $ qspec_then ‘Exp senv e2’ mp_tac
-  \\ disch_then (qspec_then ‘sk’ mp_tac)
-  \\ impl_tac
-  >- (simp [Once step_res_rel_cases]
-      \\ qexists_tac ‘0’ \\ fs [])
-  \\ rename [‘snext_res_rel xx yy’]
-  \\ simp [snext_res_rel_cases]
-  \\ strip_tac \\ fs []
-  \\ rw [] \\ gvs []
-  \\ Cases \\ fs []
-  \\ IF_CASES_TAC \\ fs []
-  \\ fs [] \\ fs [value_def] \\ rw []
-  \\ simp [sinterp_def]
-  \\ ‘compile_rel 0 (Lit (Str y)) (Lit (Str y))’ by simp [Once compile_rel_cases]
-  \\ pop_assum $ irule_at Any
-  \\ qpat_x_assum ‘cont_rel _ _ _’ $ irule_at Any \\ fs []
-  \\ ‘env_rel [] []’ by fs [env_rel_def]
-  \\ pop_assum $ irule_at Any
-  \\ first_x_assum $ irule_at Any
-  \\ simp [value_def]
-  \\ once_rewrite_tac [itreeTheory.itree_unfold_err]
-  \\ rpt conj_tac
-  \\ rpt AP_THM_TAC
-  \\ fs []
-  \\ AP_TERM_TAC
-  \\ rpt AP_THM_TAC
-  \\ AP_TERM_TAC
-  \\ once_rewrite_tac [EQ_SYM_EQ]
-  \\ irule step_unitl_halt_unwind
-  \\ fs [step_def,application_def,get_atoms_def,value_def]
-QED
-
-Theorem compile_rel_itree_of:
-  compile_rel 0 e1 e2 ⇒
-  itree_of e1 ---> itree_of e2
-Proof
-  fs [stateLangTheory.itree_of_def] \\ rw []
-  \\ irule semantics_thm
-  \\ simp [Once cont_rel_cases]
-  \\ fs [env_rel_def]
+  EVAL_TAC
 QED
 
 val _ = export_theory ();
