compiler/backend/passes/proofs/state_cexpScript.sml
@@ -1,0 +1,69 @@
+(*
+  Compiler expressions for stateLang
+*)
+open HolKernel Parse boolLib bossLib BasicProvers dep_rewrite;
+open stringTheory optionTheory sumTheory pairTheory listTheory alistTheory
+     pure_expTheory pure_semanticsTheory arithmeticTheory stateLangTheory;
+
+val _ = new_theory "state_cexp";
+
+val _ = set_grammar_ancestry ["stateLang"];
+
+val _ = numLib.prefer_num();
+
+Datatype:
+  csop = (* Primitive operations *)
+       | AppOp              (* function application                     *)
+       | Cons string        (* datatype constructor                     *)
+       | AtomOp atom_op     (* primitive parametric operator over Atoms *)
+       | Alloc              (* allocate an array                        *)
+       | Ref                (* allocates an array in a different way    *)
+       | Length             (* query the length of an array             *)
+       | Sub                (* de-reference a value in an array         *)
+       | UnsafeSub          (* de-reference but without a bounds check  *)
+       | Update             (* update a value in an array               *)
+       | UnsafeUpdate       (* update without a bounds check            *)
+       | FFI string         (* make an FFI call                         *)
+End
+
+Datatype:
+  cexp = (* stateLang expressions *)
+       | Var vname                                 (* variable                *)
+       | App csop (cexp list)                      (* application - prim/fun  *)
+       | Lam (vname option) cexp                   (* lambda                  *)
+       | Letrec ((vname # vname # cexp) list) cexp (* mutually recursive funs *)
+       | Let (vname option) cexp cexp              (* non-recursive let       *)
+       | If cexp cexp cexp                         (* if-then-else            *)
+       | Case cexp vname ((vname # vname list # cexp) list)        (* case of *)
+       | Raise cexp                                (* raise an exception      *)
+       | Handle cexp vname cexp                    (* handle an exception     *)
+       | HandleApp cexp cexp                       (* handle that takes fun   *)
+End
+
+Definition sop_of_def[simp]:
+  sop_of (AppOp:csop) = (AppOp:sop) ∧
+  sop_of (Cons n) = Cons n ∧
+  sop_of (AtomOp m) = AtomOp m ∧
+  sop_of Alloc = Alloc
+End
+
+Definition exp_of_def:
+  exp_of (Var n) = Var n ∧
+  exp_of (App op xs) = App (sop_of op) (MAP exp_of xs) ∧
+  exp_of (Lam vn x) = Lam vn (exp_of x) ∧
+  exp_of (Letrec funs x) =
+    Letrec (MAP (λ(f,v,y). (f,Lam (SOME v) (exp_of y))) funs) (exp_of x) ∧
+  exp_of (Let vn x y) = Let vn (exp_of x) (exp_of y) ∧
+  exp_of (If x y z) = If (exp_of x) (exp_of y) (exp_of z) ∧
+  exp_of (Case x v rows) =
+    Case (exp_of x) v (MAP (λ(v,vs,y). (v,vs,exp_of y)) rows) ∧
+  exp_of (Raise x) = Raise (exp_of x) ∧
+  exp_of (Handle x v y) = Handle (exp_of x) v (exp_of y) ∧
+  exp_of (HandleApp x y) = HandleApp (exp_of x) (exp_of y)
+Termination
+  WF_REL_TAC ‘measure cexp_size’
+End
+
+Theorem exp_of_def[simp] = exp_of_def |> CONV_RULE (DEPTH_CONV ETA_CONV);
+
+val _ = export_theory();
